

$$g(t) = 2$$

$$f(t) = x^2 + 1$$

$$\langle g(t), f(t) \rangle = \int_{-1}^1 g(t) \cdot f(t) dt$$

$$= \int_{-1}^1 2 \cdot (x^2 + 1) dt$$

$$= \int_{-1}^1 2x^2 + 2 dt = [\dots]_{-1}^1$$

$$= a \in \mathbb{T}_n$$

$$\begin{pmatrix} 1 \\ t \\ t^2 \end{pmatrix} \begin{matrix} f_1(t) = 1 \\ f_2(t) = t \\ f_3(t) = t^2 \end{matrix}$$

$$x_1 = \begin{pmatrix} 1 \\ 1 \\ 0 \\ 0 \end{pmatrix}, \quad x_1(t) = 1$$

$$x_2 = \begin{pmatrix} 1 \\ 0 \\ -1 \\ 1 \end{pmatrix}, \quad x_2(t) = t$$

$$x_3 = \begin{pmatrix} 0 \\ 0 \\ 1 \\ 1 \end{pmatrix}, \quad x_3(t) = t^2$$

$$\langle v_i, v_j \rangle = 0 \quad i \neq j$$

$$\langle v_i, v_i \rangle = 1$$

orange:
GS mit
Polynomen

$$1.1 \quad \tilde{v}_1 = \begin{pmatrix} 1 \\ 1 \\ 0 \\ 0 \end{pmatrix}, \quad \tilde{v}_1 \neq \underline{0}$$

$$\tilde{v}_1(t) = 1$$

$$1.2 \quad v_1 = \frac{\tilde{v}_1}{\|\tilde{v}_1\|} = \frac{1}{\sqrt{1^2 + 1^2 + 0^2 + 0^2}} \begin{pmatrix} 1 \\ 1 \\ 0 \\ 0 \end{pmatrix} = \frac{1}{\sqrt{2}} \begin{pmatrix} 1 \\ 1 \\ 0 \\ 0 \end{pmatrix}$$

$$v_1(t) = \frac{\tilde{v}_1(t)}{\|\tilde{v}_1(t)\|} = \dots = \underline{2t} \text{ (Beispiel)}$$

$$\|\tilde{v}_1(t)\| = \sqrt{\langle \tilde{v}_1(t), \tilde{v}_1(t) \rangle}$$

$$2.1 \quad \tilde{v}_2 = x_2 - \langle x_2, v_1 \rangle v_1$$

$$\tilde{v}_2(t) = t - \langle t, 2t \rangle \cdot 2t$$

$$= \begin{pmatrix} 1 \\ 0 \\ -1 \\ 1 \end{pmatrix} - \left\langle \begin{pmatrix} 1 \\ 0 \\ -1 \\ 1 \end{pmatrix}, \frac{1}{\sqrt{2}} \begin{pmatrix} 1 \\ 1 \\ 0 \\ 0 \end{pmatrix} \right\rangle \frac{1}{\sqrt{2}} \begin{pmatrix} 1 \\ 1 \\ 0 \\ 0 \end{pmatrix}$$

$$= \begin{pmatrix} 1 \\ 0 \\ -1 \\ 1 \end{pmatrix} - 1 \cdot \frac{1}{2} \begin{pmatrix} 1 \\ 1 \\ 0 \\ 0 \end{pmatrix} = \begin{pmatrix} \frac{1}{2} \\ -\frac{1}{2} \\ -1 \\ 1 \end{pmatrix} = \frac{1}{2} \begin{pmatrix} 1 \\ -1 \\ -2 \\ 2 \end{pmatrix}$$

$$2.2 \quad \tilde{v}_2 \neq \underline{0}, \quad v_2 = \frac{\tilde{v}_2}{\|\tilde{v}_2\|} = \frac{1}{\frac{1}{2} \sqrt{1^2 + (-1)^2 + (-2)^2 + 2^2}} \cdot \frac{1}{2} \begin{pmatrix} 1 \\ -1 \\ -2 \\ 2 \end{pmatrix}$$

$$= \frac{1}{\sqrt{10}} \begin{pmatrix} 1 \\ -1 \\ -2 \\ 2 \end{pmatrix}$$

$$3.1 \quad \tilde{v}_3 = x_3 - \langle x_3, v_1 \rangle v_1 - \langle x_3, v_2 \rangle v_2$$

$$= \begin{pmatrix} 0 \\ 0 \\ 1 \\ 1 \end{pmatrix} - \left\langle \begin{pmatrix} 0 \\ 0 \\ 1 \\ 1 \end{pmatrix}, \frac{1}{\sqrt{2}} \begin{pmatrix} 1 \\ 1 \\ 0 \\ 0 \end{pmatrix} \right\rangle \frac{1}{\sqrt{2}} \begin{pmatrix} 1 \\ 1 \\ 0 \\ 0 \end{pmatrix} - \left\langle \begin{pmatrix} 0 \\ 0 \\ 1 \\ 1 \end{pmatrix}, \frac{1}{\sqrt{10}} \begin{pmatrix} 1 \\ -1 \\ -2 \\ 2 \end{pmatrix} \right\rangle \frac{1}{\sqrt{10}} \begin{pmatrix} 1 \\ -1 \\ -2 \\ 2 \end{pmatrix}$$

$$= \begin{pmatrix} 0 \\ 0 \\ 1 \\ 1 \end{pmatrix}$$

$$3.2 \quad \tilde{v}_3 \neq \underline{0}, \quad v_3 = \frac{\tilde{v}_3}{\|\tilde{v}_3\|} = \frac{1}{\sqrt{2}} \begin{pmatrix} 0 \\ 0 \\ 1 \end{pmatrix}$$

$$\text{ONS} = (v_1, v_2, v_3) = \left(\frac{1}{\sqrt{2}} \begin{pmatrix} 1 \\ 1 \\ 0 \end{pmatrix}, \frac{1}{\sqrt{10}} \begin{pmatrix} 1 \\ -1 \\ 2 \end{pmatrix}, \frac{1}{\sqrt{2}} \begin{pmatrix} 0 \\ 0 \\ 1 \end{pmatrix} \right)$$

$$\mathbb{P}_{\mathbb{R}^4} \rightarrow \mathcal{W}(y) \quad y = \begin{pmatrix} 1 \\ 1 \\ 1 \\ 1 \end{pmatrix}$$

$$= \langle y, v_1 \rangle v_1 + \langle y, v_2 \rangle v_2 + \langle y, v_3 \rangle v_3$$

$$= \left\langle \begin{pmatrix} 1 \\ 1 \\ 1 \\ 1 \end{pmatrix}, \frac{1}{\sqrt{2}} \begin{pmatrix} 1 \\ 1 \\ 0 \\ 0 \end{pmatrix} \right\rangle \frac{1}{\sqrt{2}} \begin{pmatrix} 1 \\ 1 \\ 0 \\ 0 \end{pmatrix}$$

$$+ \left\langle \begin{pmatrix} 1 \\ 1 \\ 1 \\ 1 \end{pmatrix}, \frac{1}{\sqrt{10}} \begin{pmatrix} 1 \\ -1 \\ 2 \\ 2 \end{pmatrix} \right\rangle \frac{1}{\sqrt{10}} \begin{pmatrix} 1 \\ -1 \\ 2 \\ 2 \end{pmatrix}$$

$$+ \left\langle \begin{pmatrix} 1 \\ 1 \\ 1 \\ 1 \end{pmatrix}, \frac{1}{\sqrt{2}} \begin{pmatrix} 0 \\ 0 \\ 1 \\ 1 \end{pmatrix} \right\rangle \frac{1}{\sqrt{2}} \begin{pmatrix} 0 \\ 0 \\ 1 \\ 1 \end{pmatrix}$$

$$= 2 \cdot \frac{1}{2} \begin{pmatrix} 1 \\ 1 \\ 0 \\ 0 \end{pmatrix} + 0 \cdot \frac{1}{\sqrt{10}} \begin{pmatrix} 1 \\ -1 \\ 2 \\ 2 \end{pmatrix} + 2 \cdot \frac{1}{2} \begin{pmatrix} 0 \\ 0 \\ 1 \\ 1 \end{pmatrix} = \underline{\underline{\begin{pmatrix} 1 \\ 1 \\ 1 \\ 1 \end{pmatrix}}} = y$$